stdlib: set library revamped

lib/coq/set/Set.v
@@ -96,30 +96,38 @@ Definition is_empty {a:Type} {a_WT:WhyType a} (s:a -> Init.Datatypes.bool) :
   forall (x:a), ~ mem x s.
 
 (* Why3 goal *)
-Lemma mem_empty {a:Type} {a_WT:WhyType a} :
+Lemma is_empty_empty {a:Type} {a_WT:WhyType a} :
   is_empty (map.Const.const Init.Datatypes.false : a -> Init.Datatypes.bool).
 Proof.
 now intros x.
 Qed.
 
 (* Why3 goal *)
-Lemma add_spec {a:Type} {a_WT:WhyType a} :
-  forall (x:a) (s:a -> Init.Datatypes.bool), forall (y:a),
-  mem y (map.Map.set s x Init.Datatypes.true) <-> (y = x) \/ mem y s.
+Lemma empty_is_empty {a:Type} {a_WT:WhyType a} :
+  forall (s:a -> Init.Datatypes.bool), is_empty s ->
+  (s = (map.Const.const Init.Datatypes.false : a -> Init.Datatypes.bool)).
 Proof.
-intros x y s.
-unfold Map.set, mem.
-destruct why_decidable_eq ; intuition.
+intros s h1.
+apply predicate_extensionality.
+unfold is_empty in h1; unfold Const.const.
+unfold mem in h1.
+intros x. generalize (h1 x).
+destruct (s x); intuition.
 Qed.
 
 (* Why3 goal *)
-Lemma remove_spec {a:Type} {a_WT:WhyType a} :
-  forall (x:a) (s:a -> Init.Datatypes.bool), forall (y:a),
-  mem y (map.Map.set s x Init.Datatypes.false) <-> ~ (y = x) /\ mem y s.
+Lemma mem_singleton {a:Type} {a_WT:WhyType a} :
+  forall (x:a) (y:a),
+  mem y
+  (map.Map.set
+   (map.Const.const Init.Datatypes.false : a -> Init.Datatypes.bool) x
+   Init.Datatypes.true) ->
+  (y = x).
 Proof.
-intros x s y.
-unfold Map.set, mem.
-destruct why_decidable_eq ; intuition.
+intros x y h1.
+unfold mem, Map.set, Const.const in h1.
+destruct (why_decidable_eq x y) as [->|H] ; intuition.
+discriminate h1.
 Qed.
 
 (* Why3 goal *)
@@ -130,9 +138,8 @@ Lemma add_remove {a:Type} {a_WT:WhyType a} :
 Proof.
 intros x s h1.
 apply extensionality; intro y.
-rewrite add_spec.
-rewrite remove_spec.
-destruct (why_decidable_eq y x) as [->|H] ; intuition.
+unfold mem, Map.set. unfold mem in h1.
+destruct (why_decidable_eq x y) as [->|H] ; intuition.
 Qed.
 
 (* Why3 goal *)
@@ -143,10 +150,8 @@ Lemma remove_add {a:Type} {a_WT:WhyType a} :
 Proof.
 intros x s.
 apply extensionality; intro y.
-rewrite remove_spec.
-rewrite remove_spec.
-rewrite add_spec.
-destruct (why_decidable_eq y x) as [->|H] ; intuition.
+unfold mem, Map.set.
+destruct (why_decidable_eq x y) as [->|H] ; intuition.
 Qed.
 
 (* Why3 goal *)
@@ -155,8 +160,8 @@ Lemma subset_remove {a:Type} {a_WT:WhyType a} :
   subset (map.Map.set s x Init.Datatypes.false) s.
 Proof.
 intros x s y.
-rewrite remove_spec.
-now intros [_ H].
+unfold mem, Map.set.
+destruct (why_decidable_eq x y) as [->|H] ; intuition.
 Qed.
 
 (* Why3 goal *)
@@ -171,19 +176,34 @@ Defined.
 (* Why3 goal *)
 Lemma union_def {a:Type} {a_WT:WhyType a} :
   forall (s1:a -> Init.Datatypes.bool) (s2:a -> Init.Datatypes.bool) (x:a),
-  ((union s1 s2 x) = Init.Datatypes.true) <->
-  ((s1 x) = Init.Datatypes.true) \/ ((s2 x) = Init.Datatypes.true).
+  ((union s1 s2 x) = Init.Datatypes.true) <-> mem x s1 \/ mem x s2.
 Proof.
 intros s1 s2 x.
 apply Bool.orb_true_iff.
 Qed.
 
 (* Why3 goal *)
-Lemma union_spec {a:Type} {a_WT:WhyType a} :
+Lemma subset_union_1 {a:Type} {a_WT:WhyType a} :
   forall (s1:a -> Init.Datatypes.bool) (s2:a -> Init.Datatypes.bool),
-  forall (x:a), mem x (union s1 s2) <-> mem x s1 \/ mem x s2.
+  subset s1 (union s1 s2).
 Proof.
-exact union_def.
+intros s1 s2.
+unfold subset, union.
+unfold mem.
+intros x hx.
+apply Bool.orb_true_iff. intuition.
+Qed.
+
+(* Why3 goal *)
+Lemma subset_union_2 {a:Type} {a_WT:WhyType a} :
+  forall (s1:a -> Init.Datatypes.bool) (s2:a -> Init.Datatypes.bool),
+  subset s2 (union s1 s2).
+Proof.
+intros s1 s2.
+unfold subset, union.
+unfold mem.
+intros x hx.
+apply Bool.orb_true_iff. intuition.
 Qed.
 
 (* Why3 goal *)
@@ -198,19 +218,34 @@ Defined.
 (* Why3 goal *)
 Lemma inter_def {a:Type} {a_WT:WhyType a} :
   forall (s1:a -> Init.Datatypes.bool) (s2:a -> Init.Datatypes.bool) (x:a),
-  ((inter s1 s2 x) = Init.Datatypes.true) <->
-  ((s1 x) = Init.Datatypes.true) /\ ((s2 x) = Init.Datatypes.true).
+  ((inter s1 s2 x) = Init.Datatypes.true) <-> mem x s1 /\ mem x s2.
 Proof.
 intros s1 s2 x.
 apply Bool.andb_true_iff.
 Qed.
 
 (* Why3 goal *)
-Lemma inter_spec {a:Type} {a_WT:WhyType a} :
+Lemma subset_inter_1 {a:Type} {a_WT:WhyType a} :
   forall (s1:a -> Init.Datatypes.bool) (s2:a -> Init.Datatypes.bool),
-  forall (x:a), mem x (inter s1 s2) <-> mem x s1 /\ mem x s2.
+  subset (inter s1 s2) s1.
 Proof.
-exact inter_def.
+intros s1 s2.
+unfold subset, inter.
+unfold mem.
+intros x hx.
+apply Bool.andb_true_iff in hx. intuition.
+Qed.
+
+(* Why3 goal *)
+Lemma subset_inter_2 {a:Type} {a_WT:WhyType a} :
+  forall (s1:a -> Init.Datatypes.bool) (s2:a -> Init.Datatypes.bool),
+  subset (inter s1 s2) s2.
+Proof.
+intros s1 s2.
+unfold subset, inter.
+unfold mem.
+intros x hx.
+apply Bool.andb_true_iff in hx. intuition.
 Qed.
 
 (* Why3 goal *)
@@ -225,8 +260,7 @@ Defined.
 (* Why3 goal *)
 Lemma diff_def {a:Type} {a_WT:WhyType a} :
   forall (s1:a -> Init.Datatypes.bool) (s2:a -> Init.Datatypes.bool) (x:a),
-  ((diff s1 s2 x) = Init.Datatypes.true) <->
-  ((s1 x) = Init.Datatypes.true) /\ ~ ((s2 x) = Init.Datatypes.true).
+  ((diff s1 s2 x) = Init.Datatypes.true) <-> mem x s1 /\ ~ mem x s2.
 Proof.
 intros s1 s2 x.
 unfold mem, diff.
@@ -236,21 +270,13 @@ apply Bool.andb_true_iff.
 Qed.
 
 (* Why3 goal *)
-Lemma diff_spec {a:Type} {a_WT:WhyType a} :
-  forall (s1:a -> Init.Datatypes.bool) (s2:a -> Init.Datatypes.bool),
-  forall (x:a), mem x (diff s1 s2) <-> mem x s1 /\ ~ mem x s2.
-Proof.
-exact diff_def.
-Qed.
-
-(* Why3 goal *)
 Lemma subset_diff {a:Type} {a_WT:WhyType a} :
   forall (s1:a -> Init.Datatypes.bool) (s2:a -> Init.Datatypes.bool),
   subset (diff s1 s2) s1.
 Proof.
 intros s1 s2 x.
-rewrite diff_spec.
-now intros [H _].
+unfold mem.
+rewrite diff_def. intuition.
 Qed.
 
 (* Why3 goal *)
@@ -264,18 +290,16 @@ Defined.
 (* Why3 goal *)
 Lemma complement_def {a:Type} {a_WT:WhyType a} :
   forall (s:a -> Init.Datatypes.bool) (x:a),
-  ((complement s x) = Init.Datatypes.true) <->
-  ~ ((s x) = Init.Datatypes.true).
+  ((complement s x) = Init.Datatypes.true) <-> ~ mem x s.
 Proof.
 intros s x.
-unfold complement.
+unfold mem, complement.
 rewrite Bool.not_true_iff_false.
 apply Bool.negb_true_iff.
 Qed.
 
 (* Why3 goal *)
-Definition choose {a:Type} {a_WT:WhyType a} :
-  (a -> Init.Datatypes.bool) -> a.
+Definition pick {a:Type} {a_WT:WhyType a} : (a -> Init.Datatypes.bool) -> a.
 Proof.
 intros s.
 assert (i: inhabited a) by (apply inhabits, why_inhabitant).
@@ -283,12 +307,127 @@ exact (epsilon i (fun x => mem x s)).
 Defined.
 
 (* Why3 goal *)
-Lemma choose_spec {a:Type} {a_WT:WhyType a} :
-  forall (s:a -> Init.Datatypes.bool), ~ is_empty s -> mem (choose s) s.
+Lemma pick_def {a:Type} {a_WT:WhyType a} :
+  forall (s:a -> Init.Datatypes.bool), ~ is_empty s -> mem (pick s) s.
 Proof.
 intros s h1.
-unfold choose.
+unfold pick.
 apply epsilon_spec.
 now apply not_all_not_ex.
+Qed.
+
+(* Why3 assumption *)
+Definition disjoint {a:Type} {a_WT:WhyType a} (s1:a -> Init.Datatypes.bool)
+    (s2:a -> Init.Datatypes.bool) : Prop :=
+  forall (x:a), ~ mem x s1 \/ ~ mem x s2.
+
+(* Why3 goal *)
+Lemma disjoint_inter_empty {a:Type} {a_WT:WhyType a} :
+  forall (s1:a -> Init.Datatypes.bool) (s2:a -> Init.Datatypes.bool),
+  disjoint s1 s2 <-> is_empty (inter s1 s2).
+Proof.
+intros s1 s2.
+unfold disjoint, is_empty, inter.
+unfold mem.
+intuition.
+destruct (H x); intuition.
+apply H1.
+rewrite Bool.andb_true_iff in H0. intuition.
+apply H1.
+rewrite Bool.andb_true_iff in H0. intuition.
+generalize (H x).
+rewrite Bool.andb_true_iff.
+destruct (s1 x); destruct (s2 x); intuition.
+Qed.
+
+(* Why3 goal *)
+Lemma disjoint_diff_eq {a:Type} {a_WT:WhyType a} :
+  forall (s1:a -> Init.Datatypes.bool) (s2:a -> Init.Datatypes.bool),
+  disjoint s1 s2 <-> ((diff s1 s2) = s1).
+Proof.
+intros s1 s2.
+unfold disjoint, diff.
+unfold mem.
+intuition.
+apply (extensionality _ s1). unfold infix_eqeq.
+unfold mem.
+intuition.
+destruct (H x); intuition.
+rewrite Bool.andb_true_iff in H0. intuition.
+rewrite Bool.andb_true_iff in H0. intuition.
+rewrite Bool.andb_true_iff.
+intuition.
+destruct (H x); intuition.
+rewrite <- H.
+rewrite Bool.andb_true_iff.
+destruct (s2 x); intuition.
+Qed.
+
+(* Why3 goal *)
+Lemma disjoint_diff_s2 {a:Type} {a_WT:WhyType a} :
+  forall (s1:a -> Init.Datatypes.bool) (s2:a -> Init.Datatypes.bool),
+  disjoint (diff s1 s2) s2.
+Proof.
+intros s1 s2.
+unfold disjoint, diff.
+unfold mem.
+intros x.
+rewrite Bool.andb_true_iff.
+destruct (s2 x); intuition.
+Qed.
+
+(* Why3 goal *)
+Definition map {a:Type} {a_WT:WhyType a} {b:Type} {b_WT:WhyType b} :
+  (a -> b) -> (a -> Init.Datatypes.bool) -> b -> Init.Datatypes.bool.
+Proof.
+intros f s y.
+set (P := fun (x:a) => mem x s /\ y = f x).
+assert (inhabited a).
+destruct a_WT.
+exact (inhabits why_inhabitant).
+set (x := epsilon H P). 
+destruct b_WT.
+destruct (why_decidable_eq y (f x)).
+exact (s x).
+exact false.
+Defined.
+
+(* Why3 goal *)
+Lemma map_def {a:Type} {a_WT:WhyType a} {b:Type} {b_WT:WhyType b} :
+  forall (f:a -> b) (u:a -> Init.Datatypes.bool) (y:b),
+  ((map f u y) = Init.Datatypes.true) <->
+  (exists x:a, mem x u /\ (y = (f x))).
+Proof.
+intros f u y.
+unfold map, mem.
+destruct b_WT.
+destruct a_WT.
+set (P := fun (x:a) => u x = true /\ y = f x).
+set (inh := (inhabits why_inhabitant0)).
+generalize (epsilon_spec inh P).
+set (x := epsilon inh P).
+destruct (classic (exists x, P x)).
+destruct (why_decidable_eq y (f x)).
+intuition.
+unfold P in H1. intuition.
+intuition.
+unfold P in H1. intuition.
+destruct (why_decidable_eq y (f x)).
+intuition.
+exists x; unfold P; intuition.
+intuition.
+discriminate H1.
+Qed.
+
+(* Why3 goal *)
+Lemma mem_map {a:Type} {a_WT:WhyType a} {b:Type} {b_WT:WhyType b} :
+  forall (f:a -> b) (u:a -> Init.Datatypes.bool), forall (x:a), mem x u ->
+  mem (f x) (map f u).
+Proof.
+intros f u x h1.
+generalize (map_def f u (f x)).
+intuition.
+apply H1.
+exists x; intuition.
 Qed.
 
